progs/verif_logical_compare.v
@@ -1,4 +1,5 @@
 Require Import VST.floyd.proofauto.
+Require Import VST.floyd.compat.
 Require Import VST.progs.logical_compare.
 Import compcert.lib.Maps.
 
