progs/verif_ptr_compare.v
@@ -1,10 +1,9 @@
 Require Import VST.floyd.proofauto.
+Require Import VST.floyd.compat.
 Require Import VST.progs.ptr_compare.
 
 #[export] Instance CompSpecs : compspecs. make_compspecs prog. Defined.
 Definition Vprog : varspecs. mk_varspecs prog. Defined.
-
-Local Open Scope logic.
 
 Definition f_spec :=
  DECLARE _f
