progs/verif_switch.v
@@ -1,6 +1,6 @@
 Require Import VST.floyd.proofauto.
+Require Import VST.floyd.compat.
 Require Import Recdef.
-#[export] Existing Instance NullExtension.Espec.
 Require Import VST.progs.switch.
 Require Export VST.floyd.Funspec_old_Notation.
 #[export] Instance CompSpecs : compspecs. make_compspecs prog. Defined.
